enable append_right, height

test.c
@@ -1,8 +1,10 @@
 #include "P1_UInt32.c"
 
 int main() {
-  uint32_t ui = P1_UInt32_main ();
-  printf("r=%ui\n", ui);
+  uint32_t p = P1_UInt32_main ();
+  printf("r=%ui\n", p);
+  uint64_t h = P1_UInt32_main2 ();
+  printf("h=%ui\n", h);
   printf("Hello, world!\n");
   return 0;
 }
